First checker correctness theorem

Auto/Embedding/LamThm.lean
@@ -2,9 +2,33 @@ import Auto.Embedding.LamBase
 
 namespace Auto.Embedding.Lam
 
+def Eq.symm.WF (wf : LamWF ltv ⟨lctx, .app (.app (.base (.eq n)) a) b, .base .prop⟩) :
+  LamWF ltv ⟨lctx, .app (.app (.base (.eq n)) b) a, .base .prop⟩ :=
+  match wf with
+  | .ofApp argTy wfFn wfB =>
+    match wfFn with
+    | .ofApp argTy' wfEq wfA =>
+      match wfEq with
+      | .ofBase HB =>
+        match HB with
+        | .ofEq n => .ofApp _ (.ofApp _ (.ofBase (.ofEq n)) wfB) wfA
+
 theorem Eq.symm (lval : LamValuation)
   {lctxTy : Nat → LamSort} {lctxTerm : ∀ n, (lctxTy n).interp lval.ilVal.tyVal}
   (wf : LamWF lval.ilVal.toLamTyVal ⟨lctxTy, .app (.app (.base (.eq n)) a) b, .base .prop⟩)
-  (H : GLift.down (LamWF.interp lval lctxTy lctxTerm wf)) : Nat := sorry
+  (_ : GLift.down (LamWF.interp lval lctxTy lctxTerm wf)) :
+  GLift.down (LamWF.interp lval lctxTy lctxTerm (Eq.symm.WF wf)) :=
+  match wf with
+  | .ofApp argTy wfFn wfB =>
+    match wfFn with
+    | .ofApp argTy' wfEq wfA =>
+      match wfEq with
+      | .ofBase HB => by
+        cases HB; case ofEq H =>
+        dsimp [symm.WF, LamWF.interp, LamBaseWF.interp];
+        dsimp [symm.WF, LamWF.interp, LamBaseWF.interp] at H;
+        have H' := EqLift.down _ _ _ H
+        apply EqLift.up
+        exact (_root_.Eq.symm H')
 
 end Auto.Embedding.Lam
